proof-libs/fstar/rust_primitives/Rust_primitives.BitVectors.fst
@@ -1,0 +1,37 @@
+module Rust_primitives.BitVectors
+
+open FStar.Mul
+open Rust_primitives.Arrays
+open Rust_primitives.Integers
+
+#set-options "--fuel 0 --ifuel 1 --z3rlimit 40"
+
+let pow2_minus_one_mod_lemma1 (n: nat) (m: nat {m < n})
+   : Lemma (((pow2 n - 1) / pow2 m) % 2 == 1)
+   = let d: pos = n - m in
+     Math.Lemmas.pow2_plus m d;
+     Math.Lemmas.lemma_div_plus (-1) (pow2 d) (pow2 m);
+     if d > 0 then Math.Lemmas.pow2_double_mult (d-1)
+
+let pow2_minus_one_mod_lemma2 (n: nat) (m: nat {n <= m})
+  : Lemma (((pow2 n - 1) / pow2 m) % 2 == 0)
+  = Math.Lemmas.pow2_le_compat m n;
+    Math.Lemmas.small_div (pow2 n - 1) (pow2 m)
+
+let get_bit_pow2_minus_one #t n nth
+  = reveal_opaque (`%get_bit) (get_bit (mk_int #t (pow2 n - 1)) nth);
+    if v nth < n then pow2_minus_one_mod_lemma1 n (v nth)
+                 else pow2_minus_one_mod_lemma2 n (v nth)
+
+let get_bit_pow2_minus_one_i32 x nth
+  = let n = Some?.v (mask_inv_opt x) in
+    mk_int_equiv_lemma #i32_inttype x;
+    get_bit_pow2_minus_one #i32_inttype n nth
+
+let get_bit_pow2_minus_one_u8 t x nth
+  = let n = Some?.v (mask_inv_opt x) in
+    mk_int_equiv_lemma #u8_inttype x;
+    get_bit_pow2_minus_one #u8_inttype n nth
+
+let get_last_bit_signed_lemma #t x
+  = admit ()
