proof-libs/fstar/rust_primitives/Rust_primitives.Iterators.fsti
@@ -2,6 +2,7 @@ module Rust_primitives.Iterators
 
 open Rust_primitives
 open Core.Ops.Range
+open FStar.Mul
 
 val foldi_range  (#n:inttype) (#acc_t:Type)
                  (#inv:(acc_t -> i:int_t n -> Type))
